__1.__ Найти производную функции:

### $$y=\frac{1}{x}+\frac{2}{x^2}-\frac{5}{x^3}+\sqrt x -\sqrt[3]x+\frac{3}{\sqrt x}$$

Решение:

### $$y=x^{-1}+2x^{-2}-5x^{-3}+x^{\frac{1}{2}} -x^{\frac{1}{3}}+3x^{-\frac{1}{2}}$$

Тогда:

### $$y'=-x^{-2}-4x^{-3}+15x^{-4}+\frac{1}{2}x^{-\frac{1}{2}} -\frac{1}{3}x^{-\frac{2}{3}}-\frac{3}{2}x^{-\frac{3}{2}}$$


__2.__ Найти производную функции:

### $$y=x \cdot \sqrt {1+x^2}$$

Решение:

### $$y=x \cdot (1+x^2)^{\frac{1}{2}}$$

Тогда:

### $$y'=1 \cdot (1+x^2)^{\frac{1}{2}}+x \cdot \frac{1}{2}(1+x^2)^{-\frac{1}{2}}\cdot2x=\sqrt {1+x^2}+\frac{x^2}{\sqrt {1+x^2}}$$

__3.__ Найти производную функции:

### $$y= \frac{2x}{1-x^2}$$

Решение:

### $$y'= \frac{2\cdot(1-x^2)-2x\cdot(-2x)}{(1-x^2)^2}=\frac{2x^2+2}{(1-x^2)^2}$$

__5.__ Найти производную функции:

### $$y= \ln(x+\sqrt{x^2+1})$$

Решение:

### $$y'=\frac{1}{x+\sqrt{x^2+1}}\cdot \Bigr(1+\frac{x}{\sqrt{x^2+1}} \Bigl)=\frac{1}{x+\sqrt{x^2+1}}\cdot \frac{x+\sqrt{x^2+1}}{\sqrt{x^2+1}}=\frac{1}{\sqrt{x^2+1}}$$

__6.__ Найти производную функции:

### $$y=x \cdot \ln(x+\sqrt{x^2+1})-\sqrt{x^2+1}$$

Решение:

### $$y'=1 \cdot \ln(x+\sqrt{x^2+1})+x \cdot \frac{1}{\sqrt{x^2+1}}-\frac{x}{\sqrt{x^2+1}}=\ln(x+\sqrt{x^2+1})$$

